rejection_sampling.thy
@@ -1,0 +1,5 @@
+theory rejection_sampling
+  imports
+
+begin
+end
